feat: HashSet part II

lean4/ProofChecker/ProofChecker/Data/HashSet.lean
@@ -47,6 +47,11 @@ theorem not_mem_toFinset (s : HashSet α) (a : α) : a ∉ s.toFinset ↔ ¬s.co
 theorem toFinset_empty : toFinset (empty α) = ∅ := by
   ext
   simp [mem_toFinset, empty, contains, HashMap.contains_empty]
+  
+theorem toFinset_of_isEmpty (s : HashSet α) : s.isEmpty → s.toFinset = ∅ := by
+  intro h
+  ext
+  simp [mem_toFinset, contains, HashMap.not_contains_of_isEmpty _ _ h]
 
 @[simp]
 theorem toFinset_insert (s : HashSet α) (a : α) :
@@ -144,17 +149,78 @@ theorem toFinset_Union (l : Array (HashSet α)) :
 disjoint. Return `(⋃ ss, true)` if array elements are pairwise disjoint, otherwise `(⋃ ss, false)`.
 -/
 def disjointUnion (ss : Array (HashSet α)) : HashSet α × Bool :=
-  ss.foldl
-    (init := (.empty α, true))
-    fun (acc : HashSet α × Bool) t =>
-      (acc.1.union t, acc.2 && (acc.1.inter t).isEmpty)
+  ss.foldl (init := (.empty α, true)) fun (U, b) t =>
+    (U.union t, b && (U.inter t).isEmpty)
+      
+theorem disjointUnion_characterization (ss : Array (HashSet α)) :
+    (∀ a, a ∈ (disjointUnion ss).fst.toFinset ↔ ∃ s ∈ ss.data, a ∈ s.toFinset)
+    ∧ ((disjointUnion ss).snd →
+      ∀ (i j : Fin ss.size), i ≠ j → ss[i].toFinset ∩ ss[j].toFinset = ∅) :=
+  have ⟨h₁, h₂, h₃⟩ := ss.foldl_induction
+    (motive := fun i (acc : HashSet α × Bool) =>
+      (∀ a ∈ acc.1.toFinset, ∃ s ∈ ss.data, a ∈ s.toFinset) ∧
+      (∀ (j : Fin ss.size), j < i → ss[j].toFinset ⊆ acc.1.toFinset) ∧
+      (acc.2 → ∀ (j k : Fin ss.size), j < i → k < i → j ≠ k → ss[j].toFinset ∩ ss[k].toFinset = ∅))
+    (init := (empty α, true)) (h0 := by simp)
+    (f := fun acc t =>
+      (acc.1.union t, acc.2 && (acc.1.inter t).isEmpty))
+    (hf := by
+      intro i (U, b) ⟨ih₁, ih₂, ih₃⟩
+      simp only [toFinset_union, Finset.mem_union]
+      refine ⟨?step₁, ?step₂, ?step₃⟩
+      case step₁ =>
+        intro a hMem
+        cases hMem with
+        | inl h =>
+          exact ih₁ a h
+        | inr h =>
+          exact ⟨ss[i], Array.get_mem_data ss i, h⟩
+      case step₂ =>
+        intro j hJ
+        cases Nat.lt_or_eq_of_le (Nat.le_of_lt_succ hJ) with
+        | inl h =>
+          have := ih₂ j h
+          exact subset_trans this (Finset.subset_union_left _ _)
+        | inr h =>
+          simp [h, Finset.subset_union_right]
+      case step₃ =>
+        intro hB j k hJ hK hNe
+        simp only [Bool.and_eq_true] at hB
+        cases Nat.lt_or_eq_of_le (Nat.le_of_lt_succ hJ) <;>
+          cases Nat.lt_or_eq_of_le (Nat.le_of_lt_succ hK)
+        case inl.inl hJ hK =>
+          exact ih₃ hB.left j k hJ hK hNe
+        case inr.inr hJ hK =>
+          have := hJ.trans hK.symm
+          exact absurd (Fin.eq_of_val_eq this) hNe
+        case inl.inr hJ hK =>
+          have hB := toFinset_of_isEmpty _ hB.right
+          simp only [toFinset_inter] at hB
+          apply Finset.subset_empty.mp
+          have := ih₂ j hJ
+          have := Finset.inter_subset_inter_right this (u := ss[k].toFinset)
+          simp_all
+        case inr.inl hJ hK =>
+          have hB := toFinset_of_isEmpty _ hB.right
+          rw [toFinset_inter, Finset.inter_comm] at hB
+          apply Finset.subset_empty.mp
+          have := ih₂ k hK
+          have := Finset.inter_subset_inter_left this (s := ss[j].toFinset)
+          simp_all)
+  by
+    dsimp [disjointUnion]
+    refine ⟨fun a => ⟨fun hMem => h₁ a hMem, ?_⟩,
+      fun h i j hNe => h₃ h i j i.isLt j.isLt hNe⟩
+    intro ⟨s, hS, hA⟩
+    have ⟨i, hI⟩ := Array.get_of_mem_data hS
+    exact h₂ i i.isLt (hI ▸ hA)
 
 theorem mem_disjointUnion (ss : Array (HashSet α)) (a : α) :
-    a ∈ (disjointUnion ss).fst.toFinset ↔ ∃ s ∈ ss.data, a ∈ s.toFinset := by
-  sorry
+    a ∈ (disjointUnion ss).fst.toFinset ↔ ∃ s ∈ ss.data, a ∈ s.toFinset :=
+  disjointUnion_characterization ss |>.left a
 
 theorem disjoint_disjointUnion (ss : Array (HashSet α)) : (disjointUnion ss).snd →
-    ∀ (i j : Fin ss.size), i ≠ j → (ss[i]).toFinset ∩ (ss[j]).toFinset = ∅ := by
-  sorry
+    ∀ (i j : Fin ss.size), i ≠ j → ss[i].toFinset ∩ ss[j].toFinset = ∅ :=
+  disjointUnion_characterization ss |>.right
 
 end HashSet
